fs_preservation.v
@@ -1,0 +1,82 @@
+Require Import syntax.
+Require Import partial.
+Require Import heap.
+Require Import classTable.
+Require Import sframe.
+Require Import reductions.
+Require Import typing.
+Require Import namesAndTypes.
+
+Require Import preservation.
+
+Require Import wf_env.
+
+Import ConcreteEverything.
+
+Section Preservation.
+
+  Variable P: Program.
+
+  Definition subtypeP := subtype P.
+  Definition fldP := fld P.
+  Definition ftypeP := ftype P.
+  Definition t_frame1' := t_frame1 P.
+  Definition WF_Frame' := WF_Frame P.
+
+  Definition Reduction_SF' := Reduction_SF P.
+  Definition Reduction_FS' := Reduction_FS P.
+  Definition fieldsP := fields P.
+  Definition TypeChecksP := TypeChecks P.
+  Definition Heap_okP := Heap_ok P.
+
+  Notation "[ H , x , tau ## FS ]" := (WF_FS P (Some (x, tau)) H FS) (at level 0).
+  Notation "[ H ## FS ]" := (WF_FS P None H FS) (at level 0).
+
+
+
+  Theorem multiple_frame_WF_ENV_preservation :
+    forall H H' FS FS',
+      Reduction_FS' (H, FS)
+                   (H', FS') ->
+      Heap_okP H ->
+      [ H ## FS ]  ->
+      [ H' ## FS' ] * (Heap_okP H').
+
+    intros.
+    inversion X.
+    (* 4 goals,  based on reduction rule:
+     * E-frame-stack,
+     * E-return1
+     * E-return2
+     * E-open
+     *)
+
+    (* CASE E-frame-stack, 
+     * H, F -> H', F',
+     * H, F :: FS --> H', F' :: FS
+     *)
+
+    admit.
+    (* TODO put in own theorem *)
+
+
+    (* Case E-return *)
+    admit. 
+    
+    (* Case E-open-return *)
+    rewrite <- H4 in *.
+    rewrite <- H6 in *.
+    rewrite <- H5 in *.
+    clear H5 H6 H3 H1.
+    split.
+    
+    inversion X0;
+    assumption.
+    assumption.
+
+
+    (* Case E-open *)
+    admit.
+  Admitted.
+
+  
