globals.v
@@ -1,0 +1,90 @@
+Require Import syntax.
+Require Import partial.
+Require Import namesAndTypes.
+Require Import heap.
+Require Import classTable.
+Require Import wf_env.
+
+
+Import ConcreteEverything.
+
+Section Globals.
+  Variable P : Program.
+
+  Require Import Coq.Lists.List.
+
+  Print sig.
+
+  Definition global_heap_lst (lst: varDefs) : Heap_type * Gamma_type * Env_type.
+    induction lst.
+    exact (p_heap.emptyPartFunc, p_gamma.emptyPartFunc, p_env.emptyPartFunc).
+    destruct IHlst.
+    destruct p.
+    destruct a.
+    rename c into C.
+    rename h into H.
+    rename e into L.
+    rename p into Gamma.
+    set (o_fresh := ConcreteNamesAndTypes.vn.constructFresh (p_heap.domain H)).
+    destruct o_fresh as [o  o_fresh_proof].
+        
+    set (flds := fieldsList P C).
+    set (FM := p_FM.newPartFunc flds FM_null).
+    set (heapVal := obj C FM).
+    split.
+    split.
+    exact (p_heap.updatePartFunc H o heapVal ).
+    exact (p_gamma.updatePartFunc Gamma v (typt_class C)).
+    exact (p_env.updatePartFunc L v (envRef o)).
+  Defined.
+
+  Definition globalEnv (P: Program) : Heap_type * Gamma_type * Env_type  :=
+    global_heap_lst (globals P).
+
+  Theorem WF_globals:
+    let (p, L) := globalEnv P in let (H, Gamma) := p in WF_Env P H Gamma L.
+    destruct P.
+    set (P' := {|
+     classDecls := classDecls;
+     globals := globals;
+     programBody := programBody;
+     programBodyIsTerm := programBodyIsTerm |}).
+    unfold globalEnv.
+    induction (syntax.globals P').
+    simpl.
+    split.
+    intro.
+    intro.
+    simpl in H.
+    elim H.
+    intros.
+    simpl in H.    
+    simplify_eq H.
+
+    case_eq (global_heap_lst v).
+    intros.
+    destruct p.
+    rename H into hyp.
+    rename h into H; rename p into Gamma; rename e into L.
+    simpl.
+    rewrite hyp.
+    destruct a.
+    rename c into C.
+    rename v0 into x.
+    rename v into rest.
+    case_eq (ConcreteNamesAndTypes.vn.constructFresh (p_heap.domain H)).
+    intros o o_fresh.
+    intro dummy; clear dummy.
+
+    split.
+    rewrite hyp in IHv.
+    destruct IHv.
+    apply subset_preserved.
+    assumption.
+
+    (* Almost done!!! *)
+    admit.
+  Admitted.
+    
+    
+End Globals.
