ocap.v
@@ -1,0 +1,38 @@
+Require Import syntax.
+Require Import partial.
+Require Import namesAndTypes.
+Require Import classTable.
+
+Import ConcreteEverything.
+
+Section Ocap.
+  Variable P : Program.
+
+  Require Import Coq.Lists.List.
+
+  Print sig.
+
+  Definition global_heap_lst (lst: varDefs) : Heap_type * Env_type.
+    induction lst.
+    exact (p_heap.emptyPartFunc, p_env.emptyPartFunc).
+    destruct IHlst.
+    set (o_fresh := ConcreteNamesAndTypes.vn.constructFresh (p_heap.domain h)).
+    destruct o_fresh as [o  o_fresh_proof].
+    destruct a.
+    rename c into C.
+    rename h into H.
+    rename e into L.
+    set (flds := fieldsList P C).
+    set (FM := p_FM.newPartFunc flds FM_null).
+    set (heapVal := obj C FM).
+    split.
+    exact (p_heap.updatePartFunc H o heapVal ).
+
+    exact (p_env.updatePartFunc L v (envRef o)).
+  Defined.
+
+  Definition globalHeap (P: Program) : Heap_type * Env_type:=
+    global_heap_lst (globals P).
+
+  
+  
